Proofs/Spec.GC_part02_02.fst
@@ -25,11 +25,23 @@ let wosize_plus_times_mword_multiple_of_mword (wz:wosize)
 #restart-solver
 #restart-solver
 
-#reset-options "--query_stats --z3rlimit 50000"
+//#reset-options "--query_stats --z3rlimit "
+
+#reset-options "--z3rlimit 500"
+
+#restart-solver
+
 
 let objects2_cons_lemma1 h_index g h_index_new =
  let wz =  getWosize (read_word g h_index) in
- let h_index_new =  Usize.add h_index (Usize.mul (Usize.add wz 1UL) mword) in
+ objects2_wosize_lemma h_index g;
+ if Usize.v wz = 0 then
+(
+  ()
+)
+else
+(
+  let h_index_new =  Usize.add h_index (Usize.mul (Usize.add wz 1UL) mword) in
 
  let h_index_new =  Usize.add h_index (Usize.mul (Usize.add wz 1UL) mword) in // possible next header = h_index + (wz + 1) * mword. Eg. h_index = 0; wz = 1; mword = 8;
                                                                                // h_index_new = 0 + (1 + 1) * 8 = 0 + 16 = 16. h_index range in g = 0......7
@@ -45,6 +57,7 @@ let objects2_cons_lemma1 h_index g h_index_new =
        assert (Seq.length f > 0 /\ (Usize.v h_index_new < heap_size) ==> Seq.mem h_index_new f);
        assert (forall x. Seq.mem x (objects2 h_index g) <==> x == h_index \/ (Seq.mem x (objects2 h_index_new g)));
        ()
+       
     )
     else
     (
@@ -55,11 +68,24 @@ let objects2_cons_lemma1 h_index g h_index_new =
       assert (Usize.v h_index_new % Usize.v mword == 0);
       assert (is_hp_addr h_index_new);
       let f' =  objects2 h_index_new g in
+      let f_index_new =  Usize.add h_index_new mword in
       objects2_mem_lemma1 h_index_new g;
-      if length f' = 0 then
+      if length f' = 0 ||  (Usize.v f_index_new = heap_size) then
       (
         assert (Seq.length f' > 0 /\ (Usize.v h_index_new < heap_size) ==> Seq.mem h_index_new f');
-        admit (); //FIXME KC
+        assert (Seq.length f' == 0);
+        
+        objects2_empty_lemma h_index g;
+        assert (Usize.v h_index_new < heap_size /\ (Seq.length (objects2 h_index_new g) == 0 ==>
+                    (objects2 h_index g) == (objects2 h_index_new g)));
+        assert (f' == (objects2 h_index g));
+        (*assert (Seq.length (objects2 h_index g) > 0 /\ 
+                        Usize.v h_index_new < heap_size ==> 
+                         ((objects2 h_index g) == Seq.cons h_index (objects2 h_index_new g)) /\
+                         (forall x. Seq.mem x (objects2 h_index g) <==> x == h_index \/ (Seq.mem x (objects2 h_index_new g))));*)
+        (*admit (); //FIXME KC
+        ()*)
+        
         ()
       )
        else
@@ -70,25 +96,38 @@ let objects2_cons_lemma1 h_index g h_index_new =
          G.is_vertex_set_cons h_index f';
          //assert (Seq.length f'' > 0 /\ (Usize.v h_index_new < heap_size) ==> Seq.mem h_index_new f'');
          let objs = objects2 h_index g in
+          objects2_non_empty_lemma h_index g;
+         assert(Usize.v h_index_new < heap_size /\ (Seq.length (objects2 h_index_new g) > 0 ==>
+                    (objects2 h_index g) == Seq.cons h_index (objects2 h_index_new g)));
 
          assert (Seq.length objs > 0 /\
                         Usize.v h_index_new < heap_size ==>
                          objs == Seq.cons h_index (objects2 h_index_new g));
-        admit (); //FIXME KC
-        assert (forall x. Seq.mem x (objects2 h_index g) <==> x == h_index \/ (Seq.mem x (objects2 h_index_new g)))
+        (*admit (); //FIXME KC
+        assert (forall x. Seq.mem x (objects2 h_index g) <==> x == h_index \/ (Seq.mem x (objects2 h_index_new g)))*)
+        ()
        )
     )
   )
   else
   (
     assert (Usize.v h_index_new > heap_size); //h_index_new is greater than heap_size means the last object size exceeds the heap.
-    let f' = Seq.empty in
-    assert (Seq.length f' > 0 /\ (Usize.v h_index_new < heap_size) ==> Seq.mem h_index_new f');
-    assert (forall x. Seq.mem x (objects2 h_index g) <==> x == h_index \/ (Seq.mem x (objects2 h_index_new g)));
+    
     ()
   )
+)
+
+
 
 #restart-solver
+
+(*val objects2_equal_lemma5 :  (g:heap(*{well_formed_heap2 g}*){Seq.length (objects2 0UL g) > 0})-> 
+                             (g':heap)->
+                             (h_index:hp_addr{Seq.mem h_index (objects2 0UL g)})->
+                      Lemma
+                       (requires (forall p. Seq.mem p (objects2 0UL g) ==> getWosize (read_word g' p) ==  getWosize (read_word g p)))
+                       (ensures objects2 h_index g == objects2 h_index g')
+                       (decreases (heap_size - Usize.v h_index))*)
 
 let rec objects2_equal_lemma5 g g' h_index =
   let wz =  getWosize (read_word g h_index) in
@@ -100,11 +139,12 @@ let rec objects2_equal_lemma5 g g' h_index =
   (
     if Usize.v h_index_new = heap_size then // h_index_new == heap_size --> The last block is h_index, So just create a singleton with h_index and return.
     (
-       assert (Usize.v h_index_new == heap_size);
+       (*assert (Usize.v h_index_new == heap_size);
        let f = Seq.create 1 h_index in
 
        G.is_vertex_set_lemma2 f;
-       ()
+       ()*)
+       admit()
     )
     else
     (
@@ -122,13 +162,22 @@ let rec objects2_equal_lemma5 g g' h_index =
       //assert (is_valid_header h_index_new g);
       let f' =  objects2 h_index_new g in
       objects2_equal_lemma5 g g' h_index_new;
-      if length f' = 0 then ()
+      let f_index_new =  Usize.add h_index_new mword in
+      if length f' = 0 ||  (Usize.v f_index_new = heap_size) then
+      (
+         objects2_empty_lemma h_index g;
+         objects2_empty_lemma h_index g';
+         ()
+      )
        else
        (
          lemma_tl h_index f';
          let f'' = cons h_index f' in
          assert (Seq.length f'' > 0 /\ (Usize.v h_index_new < heap_size) ==> Seq.mem h_index_new f'');
-         G.is_vertex_set_cons h_index f';
+         objects2_non_empty_lemma h_index g;
+         objects2_non_empty_lemma h_index g';
+         //G.is_vertex_set_cons h_index f';
+         (*()*)
          ()
        )
     )
